\documentclass[a4j]{jarticle}
\usepackage{amsmath}
\usepackage{ascmac}
\usepackage{amssymb}
\usepackage{enumerate}
\usepackage{multicol}
\usepackage{framed}
\usepackage{latexsym}
\usepackage{indent}
\usepackage{cases}
\allowdisplaybreaks
\title{}
\begin{document}
\input{macros}
\begin{oframed}
$x_1,x_2\dots,x_n$はおのおの$0$，$1$，$2$のどれかの値を取る．$f_1=\dsum{i=1}{n}x_i$，
$f_2=\dsum{i=1}{n}x_i^2$のとき$f_k=\dsum{i=1}{n}x_i^k(k=1,2,3,\cdots)$を$f_1$と$f_2$とを用いて
表せ．
\end{oframed}

\setlength{\columnseprule}{0.4pt}
\begin{multicols}{2}
{\bf[解]}$x_i(i=1,2,\dots,n)$の中に$0$が$a$個，$1$が$b$個，$2$が$c$個あるとすると，
題意から
     \begin{align}
     a+b+c=n \\
     f_1=b+2c \label{2}\\
     f_2=b+4c  \label{3}\\
     f_k=b+2^kc \label{4}
     \end{align}
である．\eqref{2}，\eqref{3}から$b=2f_1-f_2$，$c=\dfrac{f_2-f_1}{2}$だから，これを\eqref{4}に代入して
     \begin{align*}
     f_k&=2f_1-f_2+2^k\frac{f_2-f_1}{2} \\
     &=(2-2^{k-1})f_1+(-1+2^{k-1})f_2\cdots\text{(答)}
     \end{align*}
である．         
\newpage
\end{multicols}
\end{document}